messageInvariantPrototypes/paxos/decentralizedMonotonicTemplated/messageInvariants.dfy
@@ -1,415 +1,289 @@
 include "spec.dfy"
 
-module PaxosMessageInvariants {
-
+module MessageInvariants {
 import opened Types
 import opened UtilitiesLibrary
+import opened MonotonicityLibrary
 import opened DistributedSystem
-import opened Obligations
 
-// certified self-inductive
-// Every message in the network has a valid source
-ghost predicate {:opaque} ValidMessageSrc(c: Constants, v: Variables) 
+ghost predicate SendPrepareValidity(c: Constants, v: Variables)
   requires v.WF(c)
+  requires ValidMessages(c, v)
 {
-  forall msg | msg in v.network.sentMsgs 
-  :: 
-  match msg 
-    case Prepare(bal) => c.ValidLeaderIdx(bal)
-    case Promise(_, acc, _) => c.ValidAcceptorIdx(acc)
-    case Propose(bal, _) => c.ValidLeaderIdx(bal)
-    case Accept(_, acc) => c.ValidAcceptorIdx(acc)
+  forall msg | msg in v.network.sentMsgs && msg.Prepare?
+  ::
+  (exists i ::
+    && v.ValidHistoryIdxStrict(i)
+    && LeaderHost.SendPrepare(c.leaders[msg.Src()], v.History(i).leaders[msg.Src()], v.History(i+1).leaders[msg.Src()], msg)
+  )
 }
 
-// Message bundle
-ghost predicate MessageInv(c: Constants, v: Variables) 
+ghost predicate SendProposeValidity(c: Constants, v: Variables)
+  requires v.WF(c)
+  requires ValidMessages(c, v)
+{
+  forall msg | msg in v.network.sentMsgs && msg.Propose?
+  ::
+  (exists i ::
+    && v.ValidHistoryIdxStrict(i)
+    && LeaderHost.SendPropose(c.leaders[msg.Src()], v.History(i).leaders[msg.Src()], v.History(i+1).leaders[msg.Src()], msg)
+  )
+}
+
+ghost predicate SendPromiseValidity(c: Constants, v: Variables)
+  requires v.WF(c)
+  requires ValidMessages(c, v)
+{
+  forall msg | msg in v.network.sentMsgs && msg.Promise?
+  ::
+  (exists i ::
+    && v.ValidHistoryIdxStrict(i)
+    && AcceptorHost.SendPromise(c.acceptors[msg.Src()], v.History(i).acceptors[msg.Src()], v.History(i+1).acceptors[msg.Src()], msg)
+  )
+}
+
+ghost predicate SendAcceptValidity(c: Constants, v: Variables)
+  requires v.WF(c)
+  requires ValidMessages(c, v)
+{
+  forall msg | msg in v.network.sentMsgs && msg.Accept?
+  ::
+  (exists i ::
+    && v.ValidHistoryIdxStrict(i)
+    && AcceptorHost.SendAccept(c.acceptors[msg.Src()], v.History(i).acceptors[msg.Src()], v.History(i+1).acceptors[msg.Src()], msg)
+  )
+}
+
+ghost predicate {:opaque} ReceivePromiseValidity(c: Constants, v: Variables)
+  requires v.WF(c)
+{
+  forall idx, i, acc |
+    && v.ValidHistoryIdx(i)
+    && 0 <= idx < |c.leaders|
+    && LeaderHost.ReceivePromiseTrigger(c.leaders[idx], v.History(i).leaders[idx], acc)
+  ::
+    (exists j, msg ::
+      && j < i
+      && v.ValidHistoryIdxStrict(j)
+      && msg in v.network.sentMsgs
+      && !LeaderHost.ReceivePromiseTrigger(c.leaders[idx], v.History(j).leaders[idx], acc)
+      && LeaderHost.ReceivePromiseTrigger(c.leaders[idx], v.History(j+1).leaders[idx], acc)
+      && LeaderHost.ReceivePromise(c.leaders[idx], v.History(j).leaders[idx], v.History(j+1).leaders[idx], msg)
+    )
+}
+
+ghost predicate {:opaque} ReceiveAcceptValidity(c: Constants, v: Variables)
+  requires v.WF(c)
+{
+  forall idx, i, acc, vb |
+    && v.ValidHistoryIdx(i)
+    && 0 <= idx < |c.learners|
+    && LearnerHost.ReceiveAcceptTrigger(c.learners[idx], v.History(i).learners[idx], acc,vb)
+  ::
+    (exists j, msg ::
+      && j < i
+      && v.ValidHistoryIdxStrict(j)
+      && msg in v.network.sentMsgs
+      && !LearnerHost.ReceiveAcceptTrigger(c.learners[idx], v.History(j).learners[idx], acc,vb)
+      && LearnerHost.ReceiveAcceptTrigger(c.learners[idx], v.History(j+1).learners[idx], acc,vb)
+      && LearnerHost.ReceiveAccept(c.learners[idx], v.History(j).learners[idx], v.History(j+1).learners[idx], msg)
+    )
+}
+
+ghost predicate MessageInv(c: Constants, v: Variables)
 {
   && v.WF(c)
-  && ValidHistory(c, v)
-  && ValidMessageSrc(c, v)
-  // Send Invariants
+  && ValidVariables(c, v)
   && SendPrepareValidity(c, v)
   && SendProposeValidity(c, v)
   && SendPromiseValidity(c, v)
   && SendAcceptValidity(c, v)
-  // Receive Invariants
-  && LeaderValidReceivedPromiseMsgs(c, v)
-  && LearnerValidReceivedAcceptMsgs(c, v)
+  && ReceivePromiseValidity(c, v)
+  && ReceiveAcceptValidity(c, v)
 }
 
+// Base obligation
 lemma InitImpliesMessageInv(c: Constants, v: Variables)
   requires Init(c, v)
   ensures MessageInv(c, v)
 {
-  reveal_ValidMessageSrc();
-  reveal_LeaderValidReceivedPromiseMsgs();
-  reveal_LearnerValidReceivedAcceptMsgs();
-  InitImpliesValidHistory(c, v);
+  InitImpliesValidVariables(c, v);
+  reveal_ReceivePromiseValidity();
+  reveal_ReceiveAcceptValidity();
 }
 
+// Inductive obligation
 lemma MessageInvInductive(c: Constants, v: Variables, v': Variables)
   requires MessageInv(c, v)
   requires Next(c, v, v')
   ensures MessageInv(c, v')
 {
-  InvNextValidHistory(c, v, v');
-  InvNextValidMessageSrc(c, v, v');
+  InvNextValidVariables(c, v, v');
   InvNextSendPrepareValidity(c, v, v');
   InvNextSendProposeValidity(c, v, v');
   InvNextSendPromiseValidity(c, v, v');
   InvNextSendAcceptValidity(c, v, v');
-  InvNextLeaderValidReceivedPromiseMsgs(c, v, v');
-  InvNextLearnerValidReceivedAccepts(c, v, v');
+  InvNextReceivePromiseValidity(c, v, v');
+  InvNextReceiveAcceptValidity(c, v, v');
 }
 
 /***************************************************************************************
-*                               Template Send Invariants                               *
+*                                     Aux Proofs                                       *
 ***************************************************************************************/
 
-// Every Prepare is sent according to LeaderHost.SendPrepare
-ghost predicate SendPrepareValidity(c: Constants, v: Variables)
-  requires v.WF(c)
-  requires ValidMessageSrc(c, v)
-{
-  reveal_ValidMessageSrc();
-  forall msg | IsPrepareMessage(v, msg)
-  :: 
-  (exists i ::
-      && v.ValidHistoryIdxStrict(i)
-      && LeaderHost.SendPrepare(c.leaderConstants[msg.bal], v.History(i).leaders[msg.bal], v.History(i+1).leaders[msg.bal], msg)
-  )
-}
-
-// Every Propose is sent according to LeaderHost.SendPropose
-ghost predicate SendProposeValidity(c: Constants, v: Variables)
-  requires v.WF(c)
-  requires ValidMessageSrc(c, v)
-{
-  reveal_ValidMessageSrc();
-  forall msg | IsProposeMessage(v, msg)
-  :: 
-  (exists i ::
-      && v.ValidHistoryIdxStrict(i)
-      && LeaderHost.SendPropose(c.leaderConstants[msg.bal], v.History(i).leaders[msg.bal], v.History(i+1).leaders[msg.bal], msg)
-  )
-}
-
-// Every Propose is sent according to AcceptorHost.SendPromise
-ghost predicate SendPromiseValidity(c: Constants, v: Variables)
-  requires v.WF(c)
-  requires ValidMessageSrc(c, v)
-{
-  reveal_ValidMessageSrc();
-  forall msg | IsPromiseMessage(v, msg)
-  :: 
-  (exists i ::
-      && v.ValidHistoryIdxStrict(i)
-      && AcceptorHost.SendPromise(c.acceptorConstants[msg.acc], v.History(i).acceptors[msg.acc], v.History(i+1).acceptors[msg.acc], msg)
-  )
-}
-
-// Every Accept is sent according to AcceptorHost.SendAccept
-ghost predicate SendAcceptValidity(c: Constants, v: Variables)
-  requires v.WF(c)
-  requires ValidMessageSrc(c, v)
-{
-  reveal_ValidMessageSrc();
-  forall msg | IsAcceptMessage(v, msg)
-  :: 
-  (exists i ::
-      && v.ValidHistoryIdxStrict(i)
-      && AcceptorHost.SendAccept(c.acceptorConstants[msg.acc], v.History(i).acceptors[msg.acc], v.History(i+1).acceptors[msg.acc], msg)
-  )
-}
-
-/***************************************************************************************
-*                               Custom Receive Invariants                              *
-***************************************************************************************/
-
-// certified self-inductive
-// Leader updates receivedPromises based on Promise messages
-// ghost predicate {:opaque} LeaderValidReceivedPromiseMsgs(c: Constants, v: Variables)
-//   requires v.WF(c)
-// {
-//   forall ldr, i, acc |
-//     && c.ValidLeaderIdx(ldr)
-//     && v.ValidHistoryIdx(i)
-//     && acc in v.History(i).leaders[ldr].receivedPromises
-//   :: 
-//     (exists prom :: 
-//       && IsPromiseMessage(v, prom)
-//       && prom.bal == ldr
-//       && prom.acc == acc
-//       && (prom.vbOpt.Some?
-//           ==> 
-//           && v.History(i).leaders[ldr].highestHeardBallot.Some?
-//           && prom.vbOpt.value.b <= v.History(i).leaders[ldr].highestHeardBallot.value
-//         )
-//     )
-// }
-
-// Leader updates receivedPromises based on Promise messages
-ghost predicate {:opaque} LeaderValidReceivedPromiseMsgs(c: Constants, v: Variables)
-  requires v.WF(c)
-{
-  forall idx, i, acc |
-    && v.ValidHistoryIdx(i)
-    && 0 <= idx < |c.leaderConstants|
-    && LeaderHost.ReceivePromiseTrigger(c.leaderConstants[idx], v.History(i).leaders[idx], acc)
-  :: 
-    (exists j, msg :: 
-      && j < i
-      && v.ValidHistoryIdxStrict(j)
-      && msg in v.network.sentMsgs
-      && !LeaderHost.ReceivePromiseTrigger(c.leaderConstants[idx], v.History(j).leaders[idx], acc)
-      && LeaderHost.ReceivePromiseTrigger(c.leaderConstants[idx], v.History(j+1).leaders[idx], acc)
-      && LeaderHost.ReceivePromise(c.leaderConstants[idx], v.History(j).leaders[idx], v.History(j+1).leaders[idx], msg)
-    )
-}
-
-// certified self-inductive
-// Learner updates its receivedAccepts map based on a Accept message carrying that 
-// accepted ValBal pair
-// ghost predicate {:opaque} LearnerValidReceivedAcceptMsgs(c: Constants, v: Variables) 
-//   requires v.WF(c)
-// {
-//   forall idx, vb, acc, i | 
-//     && c.ValidLearnerIdx(idx)
-//     && v.ValidHistoryIdx(i)
-//     && vb in v.History(i).learners[idx].receivedAccepts
-//     && acc in v.History(i).learners[idx].receivedAccepts[vb]
-//   ::
-//     Accept(vb, acc) in v.network.sentMsgs
-// }
-
-// Learner updates its receivedAccepts map based on a Accept message carrying that 
-// accepted ValBal pair
-ghost predicate {:opaque} LearnerValidReceivedAcceptMsgs(c: Constants, v: Variables) 
-  requires v.WF(c)
-{
-  forall idx, vb, acc, i | 
-    && c.ValidLearnerIdx(idx)
-    && v.ValidHistoryIdx(i)
-    && LearnerHost.ReceiveAcceptTrigger(c.learnerConstants[idx], v.History(i).learners[idx], acc, vb)
-  ::
-   (exists j, msg :: 
-       && j < i
-       && v.ValidHistoryIdxStrict(j)
-       && msg in v.network.sentMsgs
-       && !LearnerHost.ReceiveAcceptTrigger(c.learnerConstants[idx], v.History(j).learners[idx], acc, vb)
-       && LearnerHost.ReceiveAcceptTrigger(c.learnerConstants[idx], v.History(j+1).learners[idx], acc, vb)
-       && LearnerHost.ReceiveAccept(c.learnerConstants[idx], v.History(j).learners[idx], v.History(j+1).learners[idx], msg)
-    )
-}
-
-
-/***************************************************************************************
-*                               Proofs (how unfortunate)                               *
-***************************************************************************************/
-
-lemma InvNextValidMessageSrc(c: Constants, v: Variables, v': Variables)
-  requires v.WF(c)
-  requires ValidMessageSrc(c, v)
-  requires Next(c, v, v')
-  ensures ValidMessageSrc(c, v')
-{
-  reveal_ValidMessageSrc();
-  VariableNextProperties(c, v, v');
-}
 
 lemma InvNextSendPrepareValidity(c: Constants, v: Variables, v': Variables)
-  requires v.WF(c) && v'.WF(c)
-  requires ValidMessageSrc(c, v) && ValidMessageSrc(c, v')
+  requires v.WF(c)
+  requires ValidMessages(c, v)
   requires SendPrepareValidity(c, v)
   requires Next(c, v, v')
   ensures SendPrepareValidity(c, v')
 {
-  reveal_ValidMessageSrc();
-  forall msg | IsPrepareMessage(v', msg)
+  forall msg | msg in v'.network.sentMsgs && msg.Prepare?
   ensures
   (exists i ::
-      && v'.ValidHistoryIdxStrict(i)
-      && LeaderHost.SendPrepare(c.leaderConstants[msg.bal], v'.History(i).leaders[msg.bal], v'.History(i+1).leaders[msg.bal], msg)
+    && v'.ValidHistoryIdxStrict(i)
+    && LeaderHost.SendPrepare(c.leaders[msg.Src()], v'.History(i).leaders[msg.Src()], v'.History(i+1).leaders[msg.Src()], msg)
   ) {
-    VariableNextProperties(c, v, v');
-    if !IsPrepareMessage(v, msg) {
+    if msg !in v.network.sentMsgs {
       // witness and trigger
-      var i := |v'.history|-2;
-      assert LeaderHost.SendPrepare(c.leaderConstants[msg.bal], v'.History(i).leaders[msg.bal], v'.History(i+1).leaders[msg.bal], msg);
+      var i := |v.history|-1;
+      assert LeaderHost.SendPrepare(c.leaders[msg.Src()], v'.History(i).leaders[msg.Src()], v'.History(i+1).leaders[msg.Src()], msg);
     }
   }
 }
 
 lemma InvNextSendProposeValidity(c: Constants, v: Variables, v': Variables)
-  requires v.WF(c) && v'.WF(c)
-  requires ValidMessageSrc(c, v) && ValidMessageSrc(c, v')
+  requires v.WF(c)
+  requires ValidMessages(c, v)
   requires SendProposeValidity(c, v)
   requires Next(c, v, v')
   ensures SendProposeValidity(c, v')
 {
-  reveal_ValidMessageSrc();
-  forall msg | IsProposeMessage(v', msg)
+  forall msg | msg in v'.network.sentMsgs && msg.Propose?
   ensures
   (exists i ::
-      && v'.ValidHistoryIdxStrict(i)
-      && LeaderHost.SendPropose(c.leaderConstants[msg.bal], v'.History(i).leaders[msg.bal], v'.History(i+1).leaders[msg.bal], msg)
+    && v'.ValidHistoryIdxStrict(i)
+    && LeaderHost.SendPropose(c.leaders[msg.Src()], v'.History(i).leaders[msg.Src()], v'.History(i+1).leaders[msg.Src()], msg)
   ) {
-    VariableNextProperties(c, v, v');
-    if !IsProposeMessage(v, msg) {
+    if msg !in v.network.sentMsgs {
       // witness and trigger
-      var i := |v'.history|-2;
-      assert LeaderHost.SendPropose(c.leaderConstants[msg.bal], v'.History(i).leaders[msg.bal], v'.History(i+1).leaders[msg.bal], msg);
+      var i := |v.history|-1;
+      assert LeaderHost.SendPropose(c.leaders[msg.Src()], v'.History(i).leaders[msg.Src()], v'.History(i+1).leaders[msg.Src()], msg);
     }
   }
 }
 
 lemma InvNextSendPromiseValidity(c: Constants, v: Variables, v': Variables)
-  requires v.WF(c) && v'.WF(c)
-  requires ValidMessageSrc(c, v) && ValidMessageSrc(c, v')
+  requires v.WF(c)
+  requires ValidMessages(c, v)
   requires SendPromiseValidity(c, v)
   requires Next(c, v, v')
   ensures SendPromiseValidity(c, v')
 {
-  reveal_ValidMessageSrc();
-  forall msg | IsPromiseMessage(v', msg)
+  forall msg | msg in v'.network.sentMsgs && msg.Promise?
   ensures
   (exists i ::
-      && v'.ValidHistoryIdxStrict(i)
-      && AcceptorHost.SendPromise(c.acceptorConstants[msg.acc], v'.History(i).acceptors[msg.acc], v'.History(i+1).acceptors[msg.acc], msg)
+    && v'.ValidHistoryIdxStrict(i)
+    && AcceptorHost.SendPromise(c.acceptors[msg.Src()], v'.History(i).acceptors[msg.Src()], v'.History(i+1).acceptors[msg.Src()], msg)
   ) {
-    VariableNextProperties(c, v, v');
-    if !IsPromiseMessage(v, msg) {
+    if msg !in v.network.sentMsgs {
       // witness and trigger
-      var i := |v'.history|-2;
-      assert AcceptorHost.SendPromise(c.acceptorConstants[msg.acc], v'.History(i).acceptors[msg.acc], v'.History(i+1).acceptors[msg.acc], msg);
+      var i := |v.history|-1;
+      assert AcceptorHost.SendPromise(c.acceptors[msg.Src()], v'.History(i).acceptors[msg.Src()], v'.History(i+1).acceptors[msg.Src()], msg);
     }
   }
 }
 
 lemma InvNextSendAcceptValidity(c: Constants, v: Variables, v': Variables)
   requires v.WF(c)
-  requires ValidMessageSrc(c, v)
+  requires ValidMessages(c, v)
   requires SendAcceptValidity(c, v)
   requires Next(c, v, v')
   ensures SendAcceptValidity(c, v')
 {
-  reveal_ValidMessageSrc();
-  forall msg | IsAcceptMessage(v', msg)
+  forall msg | msg in v'.network.sentMsgs && msg.Accept?
   ensures
   (exists i ::
-      && v'.ValidHistoryIdxStrict(i)
-      && AcceptorHost.SendAccept(c.acceptorConstants[msg.acc], v'.History(i).acceptors[msg.acc], v'.History(i+1).acceptors[msg.acc], msg)
+    && v'.ValidHistoryIdxStrict(i)
+    && AcceptorHost.SendAccept(c.acceptors[msg.Src()], v'.History(i).acceptors[msg.Src()], v'.History(i+1).acceptors[msg.Src()], msg)
   ) {
-    VariableNextProperties(c, v, v');
-    if !IsAcceptMessage(v, msg) {
+    if msg !in v.network.sentMsgs {
       // witness and trigger
-      var i := |v'.history|-2;
-      assert AcceptorHost.SendAccept(c.acceptorConstants[msg.acc], v'.History(i).acceptors[msg.acc], v'.History(i+1).acceptors[msg.acc], msg);
+      var i := |v.history|-1;
+      assert AcceptorHost.SendAccept(c.acceptors[msg.Src()], v'.History(i).acceptors[msg.Src()], v'.History(i+1).acceptors[msg.Src()], msg);
     }
   }
 }
 
-lemma InvNextLearnerValidReceivedAccepts(c: Constants, v: Variables, v': Variables)
+lemma InvNextReceivePromiseValidity(c: Constants, v: Variables, v': Variables)
   requires v.WF(c)
-  requires LearnerValidReceivedAcceptMsgs(c, v)
+  requires ReceivePromiseValidity(c, v)
   requires Next(c, v, v')
-  ensures LearnerValidReceivedAcceptMsgs(c, v')
+  ensures ReceivePromiseValidity(c, v')
 {
-  reveal_LearnerValidReceivedAcceptMsgs();
-  forall idx, vb, acc, i |
-    && 0 <= idx < |c.learnerConstants|
-    && v'.ValidHistoryIdx(i)
-    && LearnerHost.ReceiveAcceptTrigger(c.learnerConstants[idx], v'.History(i).learners[idx], acc, vb)
-  ensures
-    (exists j, msg :: 
-      && j < i
-      && v'.ValidHistoryIdxStrict(j)
-      && msg in v'.network.sentMsgs
-      && !LearnerHost.ReceiveAcceptTrigger(c.learnerConstants[idx], v'.History(j).learners[idx], acc, vb)
-      && LearnerHost.ReceiveAcceptTrigger(c.learnerConstants[idx], v'.History(j+1).learners[idx], acc, vb)
-      && LearnerHost.ReceiveAccept(c.learnerConstants[idx], v'.History(j).learners[idx], v'.History(j+1).learners[idx], msg)
-    )
-  {
-    VariableNextProperties(c, v, v');
-    if i == |v'.history| - 1 {
-      if !LearnerHost.ReceiveAcceptTrigger(c.learnerConstants[idx], v.Last().learners[idx], acc, vb) {
-        // witnesses and triggers
-        var j := |v.history|-1;
-        var dsStep :| NextStep(c, v.Last(), v'.Last(), v.network, v'.network, dsStep);
-        var msg := dsStep.msgOps.recv.value;
-        assert LearnerHost.ReceiveAccept(c.learnerConstants[idx], v'.History(j).learners[idx], v'.History(j+1).learners[idx], msg);
-      }
-    }
-  }
-}
-
-lemma InvNextLeaderValidReceivedPromiseMsgs(c: Constants, v: Variables, v': Variables)
-  requires v.WF(c)
-  requires LeaderValidReceivedPromiseMsgs(c, v)
-  requires Next(c, v, v')
-  ensures LeaderValidReceivedPromiseMsgs(c, v')
-{
-  reveal_LeaderValidReceivedPromiseMsgs();
+  reveal_ReceivePromiseValidity();
   forall idx, i, acc |
     && v'.ValidHistoryIdx(i)
-    && 0 <= idx < |c.leaderConstants|
-    && LeaderHost.ReceivePromiseTrigger(c.leaderConstants[idx], v'.History(i).leaders[idx], acc)
+    && 0 <= idx < |c.leaders|
+    && LeaderHost.ReceivePromiseTrigger(c.leaders[idx], v'.History(i).leaders[idx], acc)
   ensures
-    (exists j, msg :: 
+    (exists j, msg ::
       && j < i
       && v'.ValidHistoryIdxStrict(j)
-      && msg in v'.network.sentMsgs
-      && !LeaderHost.ReceivePromiseTrigger(c.leaderConstants[idx], v'.History(j).leaders[idx], acc)
-      && LeaderHost.ReceivePromiseTrigger(c.leaderConstants[idx], v'.History(j+1).leaders[idx], acc)
-      && LeaderHost.ReceivePromise(c.leaderConstants[idx], v'.History(j).leaders[idx], v'.History(j+1).leaders[idx], msg)
+      && msg in v.network.sentMsgs
+      && !LeaderHost.ReceivePromiseTrigger(c.leaders[idx], v'.History(j).leaders[idx], acc)
+      && LeaderHost.ReceivePromiseTrigger(c.leaders[idx], v'.History(j+1).leaders[idx], acc)
+      && LeaderHost.ReceivePromise(c.leaders[idx], v'.History(j).leaders[idx], v'.History(j+1).leaders[idx], msg)
     )
   {
     VariableNextProperties(c, v, v');
     if i == |v'.history| - 1 {
-      if !LeaderHost.ReceivePromiseTrigger(c.leaderConstants[idx], v.Last().leaders[idx], acc) {
-        // witnesses and triggers
+      if !LeaderHost.ReceivePromiseTrigger(c.leaders[idx], v.Last().leaders[idx], acc)
+      {
+        // witness and triggers
         var j := |v.history|-1;
         var dsStep :| NextStep(c, v.Last(), v'.Last(), v.network, v'.network, dsStep);
         var msg := dsStep.msgOps.recv.value;
-        assert LeaderHost.ReceivePromise(c.leaderConstants[idx], v'.History(j).leaders[idx], v'.History(j+1).leaders[idx], msg);
+        assert LeaderHost.ReceivePromise(c.leaders[idx], v'.History(j).leaders[idx], v'.History(j+1).leaders[idx], msg);
       }
     }
   }
 }
 
-/***************************************************************************************
-*                                        Utils                                         *
-***************************************************************************************/
-
-ghost predicate IsPrepareMessage(v: Variables, m: Message) {
-  && m.Prepare?
-  && m in v.network.sentMsgs
-}
-
-ghost predicate IsPromiseMessage(v: Variables, m: Message) {
-  && m.Promise?
-  && m in v.network.sentMsgs
-}
-
-ghost predicate IsProposeMessage(v: Variables, m: Message) {
-  && m.Propose?
-  && m in v.network.sentMsgs
-}
-
-ghost predicate IsAcceptMessage(v: Variables, m: Message) {
-  && m.Accept?
-  && m in v.network.sentMsgs
-}
-
-lemma GetAcceptorSet(c: Constants, v: Variables)
-returns (accSet: set<AcceptorId>)
+lemma InvNextReceiveAcceptValidity(c: Constants, v: Variables, v': Variables)
   requires v.WF(c)
-  ensures forall a :: c.ValidAcceptorIdx(a) <==> a in accSet
-  ensures |accSet| == 2 * c.f + 1
+  requires ReceiveAcceptValidity(c, v)
+  requires Next(c, v, v')
+  ensures ReceiveAcceptValidity(c, v')
 {
-  assert v.History(0).WF(c);  // trigger for |c.acceptorConstants| == 2 * c.f+1
-  accSet := set a |  0 <= a < |c.acceptorConstants|;
-  SetComprehensionSize(|c.acceptorConstants|);
+  reveal_ReceiveAcceptValidity();
+  forall idx, i, acc, vb |
+    && v'.ValidHistoryIdx(i)
+    && 0 <= idx < |c.learners|
+    && LearnerHost.ReceiveAcceptTrigger(c.learners[idx], v'.History(i).learners[idx], acc,vb)
+  ensures
+    (exists j, msg ::
+      && j < i
+      && v'.ValidHistoryIdxStrict(j)
+      && msg in v.network.sentMsgs
+      && !LearnerHost.ReceiveAcceptTrigger(c.learners[idx], v'.History(j).learners[idx], acc,vb)
+      && LearnerHost.ReceiveAcceptTrigger(c.learners[idx], v'.History(j+1).learners[idx], acc,vb)
+      && LearnerHost.ReceiveAccept(c.learners[idx], v'.History(j).learners[idx], v'.History(j+1).learners[idx], msg)
+    )
+  {
+    VariableNextProperties(c, v, v');
+    if i == |v'.history| - 1 {
+      if !LearnerHost.ReceiveAcceptTrigger(c.learners[idx], v.Last().learners[idx], acc,vb)
+      {
+        // witness and triggers
+        var j := |v.history|-1;
+        var dsStep :| NextStep(c, v.Last(), v'.Last(), v.network, v'.network, dsStep);
+        var msg := dsStep.msgOps.recv.value;
+        assert LearnerHost.ReceiveAccept(c.learners[idx], v'.History(j).learners[idx], v'.History(j+1).learners[idx], msg);
+      }
+    }
+  }
 }
-}  // end module PaxosProof
 
+} // end module MessageInvariants
